coq/JsSyntaxInfos.v
@@ -1,0 +1,99 @@
+Require Import JsSyntax JsSyntaxAux.
+
+
+(**************************************************************)
+(** ** Implicit Types *)
+
+Implicit Type e : expr.
+Implicit Type p : prog.
+Implicit Type t : stat.
+
+Implicit Type fb : funcbody.
+Implicit Type el : element.
+Implicit Type str : strictness_flag.
+
+
+(**************************************************************)
+(** Annotate the AST of a program with label sets (used for
+    break and continue), and propagate strictness information
+    downwards in the AST (so that any function code under a
+    strictness directive will be tagged as strict). Note 
+    that label sets only accumulate at the head of loop 
+    statements. *)
+
+(** Propagate through expressions *)
+
+Fixpoint add_infos_exp str e :=
+   let f := add_infos_exp str in
+   match e with
+     | expr_this 
+     | expr_identifier _
+     | expr_literal _
+     | expr_object _ => e
+     | expr_function so ss fb => expr_function so ss (add_infos_funcbody str fb)
+     | expr_access e1 e2 => expr_access (f e1) (f e2)
+     | expr_member e s => expr_member (f e) s
+     | expr_new e es => expr_new (f e) (List.map f es)
+     | expr_call e es => expr_call (f e) (List.map f es)
+     | expr_unary_op op e => expr_unary_op op (f e)
+     | expr_binary_op e1 op e2 => expr_binary_op (f e1) op (f e2)
+     | expr_conditional e1 e2 e3 => expr_conditional (f e1) (f e2) (f e3)
+     | expr_assign e1 op e2 => expr_assign (f e1) op (f e2)
+   end
+   
+(** Propagate through function bodies *)
+
+with add_infos_funcbody str fb :=
+   match fb with
+     | funcbody_intro p s => funcbody_intro (add_infos_prog str p) s
+   end
+
+(** Propagate through statments *)
+
+with add_infos_stat str labs t :=
+  let opt {A} (f : A -> A) (smth : option A) :=
+    match smth with
+      | Some smth => Some (f smth)
+      | None => None
+    end in
+  let f := add_infos_stat str label_set_empty in
+  let fo := opt f in
+  let fe := add_infos_exp str in
+  let feo := opt fe in
+  match t with 
+    | stat_expr e => stat_expr (fe e)
+    | stat_label l t => stat_label l (add_infos_stat str (label_set_add l labs) t)
+    | stat_block ts => stat_block (List.map f ts)
+    | stat_var_decl vars => stat_var_decl (List.map (fun var =>
+        let '(s, eo) := var in (s, feo eo)) vars)
+    | stat_if e t to => stat_if (fe e) (f t) (fo to) 
+    | stat_do_while _ t e => stat_do_while (label_set_add_empty labs) (f t) (fe e)
+    | stat_while _ e t => stat_while (label_set_add_empty labs) (fe e) (f t)
+    | stat_with e t => stat_with (fe e) (f t)
+    | stat_throw e => stat_throw (fe e)
+    | stat_return eo => stat_return (feo eo)
+    | stat_break lopt => stat_break lopt
+    | stat_continue lopt => stat_continue lopt
+    | stat_try t catch to =>
+      stat_try (f t) (opt (fun c => let '(cs, t) := c in (cs, f t)) catch) (fo to) 
+    | stat_for_in _ e1 e2 t => stat_for_in (label_set_add_empty labs) (fe e1) (fe e2) (f t)
+    | stat_for_in_var _ str eo e t => stat_for_in_var (label_set_add_empty labs) str (feo eo) (fe e) (f t)
+    | stat_debugger => stat_debugger
+  end
+
+(** Propagate through programs *)
+
+with add_infos_prog str p :=
+  match p with
+    | prog_intro str' els =>  
+      let str'' := (str || str') in
+      prog_intro str'' (List.map (add_infos_element str'') els)
+  end
+ 
+(** Propagate through program elements *)
+
+with add_infos_element str el :=
+  match el with
+    | element_stat t => element_stat (add_infos_stat str label_set_empty t)
+    | element_func_decl s ss fb => element_func_decl s ss (add_infos_funcbody str fb)
+  end.
